Semantics/I_Seq_Semantics.thy
@@ -2,26 +2,73 @@ theory I_Seq_Semantics
   imports I_Semantics Seq_Semantics
 begin
 
-locale I_Seq_Semantics = I_Semantics_Sig + Seq_Semantics_Sig
+locale I_Seq_Semantics_Sig = I_Semantics_Sig + Seq_Semantics_Sig
+
+locale I_Seq_Semantics = I_Seq_Semantics_Sig
 
 sublocale I_Semantics \<subseteq> Base_Next_Semantics
-  where base_sem = i_base_sem
+  where xr = xr
+  and ms = ms
+  and base_sem = i_base_sem
   done
 
 
 sublocale I_Seq_Semantics \<subseteq> I_Semantics
-  where i_sem = i_sem
+  where xr = xr
+  and ms = ms
+  and i_sem = i_sem
   done
 
 sublocale I_Seq_Semantics \<subseteq> Seq_Semantics
-  where seq_sem = seq_sem
+  where xr = xr
+  and ms = ms
+  and seq_sem = seq_sem
   done
 
+(* problem now is with merging the states *)
 
-print_locale! I_Seq_Semantics
+locale I_Seq_Semantics_Final = I_Seq_Semantics
 
-sublocale I_Seq_Semantics \<subseteq> Gensyn_Semantics
-  where base_sem = i_base_sem
-    and rec_sem = seq_rec_sem
+sublocale I_Seq_Semantics_Final \<subseteq> Gensyn_Semantics
+  where xr = xr
+  and ms = ms
+  and base_sem = base_sem_next
+  and rec_sem = seq_rec_sem
+  done
+
+print_locale I_Seq_Semantics
+
+interpretation Gensyn_Semantics_Seq_Calc :
+  I_Seq_Semantics_Final "TYPE(unit)" _ calc_semb seq_nop
+  done
+term "Gensyn_Semantics_Seq_Calc.gensyn_sem"
+
+lemma testout2 : "Gensyn_Semantics_Seq_Calc.gensyn_sem (GRec () (LSeq ()) [(GBase () (LInst AccReset))
+                                                                         ,(GBase () (LInst (AccAdd 1)))]) [] 0 43"
+  
+  apply(fastforce intro : Gensyn_Semantics_Seq_Calc.gensyn_sem.intros
+Gensyn_Semantics_Seq_Calc.seq_rec_sem.intros
+seq_nop.intros
+I_Semantics_Calc.base_sem_next.intros
+I_Semantics_Calc.i_base_sem.intros
+calc_semb.intros)
+
+(*  
+  apply(rule Gensyn_Semantics_Seq_Calc.gensyn_sem.intros(4)) apply(auto)
+   apply(rule "Gensyn_Semantics_Seq_Calc.seq_rec_sem.intros") apply(auto)
+   apply(rule "seq_nop.intros")
+  apply(rule "Gensyn_Semantics_Seq_Calc.gensyn_sem.intros"(2))
+    apply(auto)
+   apply(rule "I_Semantics_Calc.base_sem_next.intros") apply(auto)
+   apply(rule "I_Semantics_Calc.i_base_sem.intros")
+   apply(rule "calc_semb.intros") apply(auto)
+  apply(rule "Gensyn_Semantics_Seq_Calc.gensyn_sem.intros"(1))
+   apply(auto)
+  apply(rule "I_Semantics_Calc.base_sem_next.intros"(2)) apply(auto)
+  apply(rule "I_Semantics_Calc.i_base_sem.intros")
+  apply(rule "calc_semb.intros") apply(auto)
+*)
+  done
+
 
 end
